wip

ocaml/fstar-lib/generated/FStar_Tactics_V2_Interpreter.ml
@@ -1895,8 +1895,13 @@ let (uu___193 : unit) =
                                                                     =
                                                                     let uu___174
                                                                     =
+                                                                    let uu___175
+                                                                    =
+                                                                    FStar_Syntax_Embeddings.e_tuple2
+                                                                    FStar_Tactics_Embedding.e_tot_or_ghost
+                                                                    FStar_Reflection_V2_Embeddings.e_term in
                                                                     FStar_Syntax_Embeddings.e_option
-                                                                    FStar_Syntax_Embeddings.e_unit in
+                                                                    uu___175 in
                                                                     let uu___175
                                                                     =
                                                                     FStar_Syntax_Embeddings.e_list
@@ -1908,8 +1913,13 @@ let (uu___193 : unit) =
                                                                     =
                                                                     let uu___175
                                                                     =
+                                                                    let uu___176
+                                                                    =
+                                                                    FStar_TypeChecker_NBETerm.e_tuple2
+                                                                    FStar_Tactics_Embedding.e_tot_or_ghost_nbe
+                                                                    FStar_Reflection_V2_NBEEmbeddings.e_term in
                                                                     FStar_TypeChecker_NBETerm.e_option
-                                                                    FStar_TypeChecker_NBETerm.e_unit in
+                                                                    uu___176 in
                                                                     let uu___176
                                                                     =
                                                                     FStar_TypeChecker_NBETerm.e_list
@@ -1917,20 +1927,16 @@ let (uu___193 : unit) =
                                                                     FStar_TypeChecker_NBETerm.e_tuple2
                                                                     uu___175
                                                                     uu___176 in
-                                                                    FStar_Tactics_V2_InterpFuns.mk_tac_step_4
+                                                                    FStar_Tactics_V2_InterpFuns.mk_tac_step_2
                                                                     Prims.int_zero
-                                                                    "core_check_term"
-                                                                    FStar_Tactics_V2_Basic.refl_core_check_term
+                                                                    "core_compute_term_type2"
+                                                                    FStar_Tactics_V2_Basic.refl_core_compute_term_type2
                                                                     FStar_Reflection_V2_Embeddings.e_env
                                                                     FStar_Reflection_V2_Embeddings.e_term
-                                                                    FStar_Reflection_V2_Embeddings.e_term
-                                                                    FStar_Tactics_Embedding.e_tot_or_ghost
                                                                     uu___173
-                                                                    FStar_Tactics_V2_Basic.refl_core_check_term
+                                                                    FStar_Tactics_V2_Basic.refl_core_compute_term_type2
                                                                     FStar_Reflection_V2_NBEEmbeddings.e_env
                                                                     FStar_Reflection_V2_NBEEmbeddings.e_term
-                                                                    FStar_Reflection_V2_NBEEmbeddings.e_term
-                                                                    FStar_Tactics_Embedding.e_tot_or_ghost_nbe
                                                                     uu___174 in
                                                                     let uu___173
                                                                     =
@@ -1940,13 +1946,8 @@ let (uu___193 : unit) =
                                                                     =
                                                                     let uu___176
                                                                     =
-                                                                    let uu___177
-                                                                    =
-                                                                    FStar_Syntax_Embeddings.e_tuple2
-                                                                    FStar_Reflection_V2_Embeddings.e_term
-                                                                    FStar_Reflection_V2_Embeddings.e_term in
                                                                     FStar_Syntax_Embeddings.e_option
-                                                                    uu___177 in
+                                                                    FStar_Syntax_Embeddings.e_unit in
                                                                     let uu___177
                                                                     =
                                                                     FStar_Syntax_Embeddings.e_list
@@ -1958,13 +1959,8 @@ let (uu___193 : unit) =
                                                                     =
                                                                     let uu___177
                                                                     =
-                                                                    let uu___178
-                                                                    =
-                                                                    FStar_TypeChecker_NBETerm.e_tuple2
-                                                                    FStar_Reflection_V2_NBEEmbeddings.e_term
-                                                                    FStar_Reflection_V2_NBEEmbeddings.e_term in
                                                                     FStar_TypeChecker_NBETerm.e_option
-                                                                    uu___178 in
+                                                                    FStar_TypeChecker_NBETerm.e_unit in
                                                                     let uu___178
                                                                     =
                                                                     FStar_TypeChecker_NBETerm.e_list
@@ -1972,16 +1968,18 @@ let (uu___193 : unit) =
                                                                     FStar_TypeChecker_NBETerm.e_tuple2
                                                                     uu___177
                                                                     uu___178 in
-                                                                    FStar_Tactics_V2_InterpFuns.mk_tac_step_3
+                                                                    FStar_Tactics_V2_InterpFuns.mk_tac_step_4
                                                                     Prims.int_zero
-                                                                    "tc_term"
-                                                                    FStar_Tactics_V2_Basic.refl_tc_term
+                                                                    "core_check_term"
+                                                                    FStar_Tactics_V2_Basic.refl_core_check_term
                                                                     FStar_Reflection_V2_Embeddings.e_env
+                                                                    FStar_Reflection_V2_Embeddings.e_term
                                                                     FStar_Reflection_V2_Embeddings.e_term
                                                                     FStar_Tactics_Embedding.e_tot_or_ghost
                                                                     uu___175
-                                                                    FStar_Tactics_V2_Basic.refl_tc_term
+                                                                    FStar_Tactics_V2_Basic.refl_core_check_term
                                                                     FStar_Reflection_V2_NBEEmbeddings.e_env
+                                                                    FStar_Reflection_V2_NBEEmbeddings.e_term
                                                                     FStar_Reflection_V2_NBEEmbeddings.e_term
                                                                     FStar_Tactics_Embedding.e_tot_or_ghost_nbe
                                                                     uu___176 in
@@ -1993,8 +1991,13 @@ let (uu___193 : unit) =
                                                                     =
                                                                     let uu___178
                                                                     =
+                                                                    let uu___179
+                                                                    =
+                                                                    FStar_Syntax_Embeddings.e_tuple2
+                                                                    FStar_Reflection_V2_Embeddings.e_term
+                                                                    FStar_Reflection_V2_Embeddings.e_term in
                                                                     FStar_Syntax_Embeddings.e_option
-                                                                    FStar_Reflection_V2_Embeddings.e_universe in
+                                                                    uu___179 in
                                                                     let uu___179
                                                                     =
                                                                     FStar_Syntax_Embeddings.e_list
@@ -2006,8 +2009,13 @@ let (uu___193 : unit) =
                                                                     =
                                                                     let uu___179
                                                                     =
+                                                                    let uu___180
+                                                                    =
+                                                                    FStar_TypeChecker_NBETerm.e_tuple2
+                                                                    FStar_Reflection_V2_NBEEmbeddings.e_term
+                                                                    FStar_Reflection_V2_NBEEmbeddings.e_term in
                                                                     FStar_TypeChecker_NBETerm.e_option
-                                                                    FStar_Reflection_V2_NBEEmbeddings.e_universe in
+                                                                    uu___180 in
                                                                     let uu___180
                                                                     =
                                                                     FStar_TypeChecker_NBETerm.e_list
@@ -2015,16 +2023,18 @@ let (uu___193 : unit) =
                                                                     FStar_TypeChecker_NBETerm.e_tuple2
                                                                     uu___179
                                                                     uu___180 in
-                                                                    FStar_Tactics_V2_InterpFuns.mk_tac_step_2
+                                                                    FStar_Tactics_V2_InterpFuns.mk_tac_step_3
                                                                     Prims.int_zero
-                                                                    "universe_of"
-                                                                    FStar_Tactics_V2_Basic.refl_universe_of
+                                                                    "tc_term"
+                                                                    FStar_Tactics_V2_Basic.refl_tc_term
                                                                     FStar_Reflection_V2_Embeddings.e_env
                                                                     FStar_Reflection_V2_Embeddings.e_term
+                                                                    FStar_Tactics_Embedding.e_tot_or_ghost
                                                                     uu___177
-                                                                    FStar_Tactics_V2_Basic.refl_universe_of
+                                                                    FStar_Tactics_V2_Basic.refl_tc_term
                                                                     FStar_Reflection_V2_NBEEmbeddings.e_env
                                                                     FStar_Reflection_V2_NBEEmbeddings.e_term
+                                                                    FStar_Tactics_Embedding.e_tot_or_ghost_nbe
                                                                     uu___178 in
                                                                     let uu___177
                                                                     =
@@ -2034,8 +2044,18 @@ let (uu___193 : unit) =
                                                                     =
                                                                     let uu___180
                                                                     =
+                                                                    let uu___181
+                                                                    =
+                                                                    let uu___182
+                                                                    =
+                                                                    FStar_Syntax_Embeddings.e_tuple2
+                                                                    FStar_Tactics_Embedding.e_tot_or_ghost
+                                                                    FStar_Reflection_V2_Embeddings.e_term in
+                                                                    FStar_Syntax_Embeddings.e_tuple2
+                                                                    FStar_Reflection_V2_Embeddings.e_term
+                                                                    uu___182 in
                                                                     FStar_Syntax_Embeddings.e_option
-                                                                    FStar_Syntax_Embeddings.e_unit in
+                                                                    uu___181 in
                                                                     let uu___181
                                                                     =
                                                                     FStar_Syntax_Embeddings.e_list
@@ -2047,8 +2067,18 @@ let (uu___193 : unit) =
                                                                     =
                                                                     let uu___181
                                                                     =
+                                                                    let uu___182
+                                                                    =
+                                                                    let uu___183
+                                                                    =
+                                                                    FStar_TypeChecker_NBETerm.e_tuple2
+                                                                    FStar_Tactics_Embedding.e_tot_or_ghost_nbe
+                                                                    FStar_Reflection_V2_NBEEmbeddings.e_term in
+                                                                    FStar_TypeChecker_NBETerm.e_tuple2
+                                                                    FStar_Reflection_V2_NBEEmbeddings.e_term
+                                                                    uu___183 in
                                                                     FStar_TypeChecker_NBETerm.e_option
-                                                                    FStar_TypeChecker_NBETerm.e_unit in
+                                                                    uu___182 in
                                                                     let uu___182
                                                                     =
                                                                     FStar_TypeChecker_NBETerm.e_list
@@ -2058,12 +2088,12 @@ let (uu___193 : unit) =
                                                                     uu___182 in
                                                                     FStar_Tactics_V2_InterpFuns.mk_tac_step_2
                                                                     Prims.int_zero
-                                                                    "check_prop_validity"
-                                                                    FStar_Tactics_V2_Basic.refl_check_prop_validity
+                                                                    "tc_term2"
+                                                                    FStar_Tactics_V2_Basic.refl_tc_term2
                                                                     FStar_Reflection_V2_Embeddings.e_env
                                                                     FStar_Reflection_V2_Embeddings.e_term
                                                                     uu___179
-                                                                    FStar_Tactics_V2_Basic.refl_check_prop_validity
+                                                                    FStar_Tactics_V2_Basic.refl_tc_term2
                                                                     FStar_Reflection_V2_NBEEmbeddings.e_env
                                                                     FStar_Reflection_V2_NBEEmbeddings.e_term
                                                                     uu___180 in
@@ -2073,69 +2103,41 @@ let (uu___193 : unit) =
                                                                     =
                                                                     let uu___181
                                                                     =
+                                                                    let uu___182
+                                                                    =
+                                                                    FStar_Syntax_Embeddings.e_option
+                                                                    FStar_Reflection_V2_Embeddings.e_universe in
+                                                                    let uu___183
+                                                                    =
                                                                     FStar_Syntax_Embeddings.e_list
-                                                                    FStar_Reflection_V2_Embeddings.e_pattern in
+                                                                    FStar_Syntax_Embeddings.e_issue in
+                                                                    FStar_Syntax_Embeddings.e_tuple2
+                                                                    uu___182
+                                                                    uu___183 in
                                                                     let uu___182
                                                                     =
                                                                     let uu___183
                                                                     =
-                                                                    let uu___184
-                                                                    =
-                                                                    FStar_Syntax_Embeddings.e_list
-                                                                    FStar_Reflection_V2_Embeddings.e_pattern in
-                                                                    let uu___185
-                                                                    =
-                                                                    let uu___186
-                                                                    =
-                                                                    FStar_Syntax_Embeddings.e_list
-                                                                    FStar_Reflection_V2_Embeddings.e_binding in
-                                                                    FStar_Syntax_Embeddings.e_list
-                                                                    uu___186 in
-                                                                    FStar_Syntax_Embeddings.e_tuple2
-                                                                    uu___184
-                                                                    uu___185 in
-                                                                    FStar_Syntax_Embeddings.e_option
-                                                                    uu___183 in
-                                                                    let uu___183
-                                                                    =
-                                                                    FStar_TypeChecker_NBETerm.e_list
-                                                                    FStar_Reflection_V2_NBEEmbeddings.e_pattern in
-                                                                    let uu___184
-                                                                    =
-                                                                    let uu___185
-                                                                    =
-                                                                    let uu___186
-                                                                    =
-                                                                    FStar_TypeChecker_NBETerm.e_list
-                                                                    FStar_Reflection_V2_NBEEmbeddings.e_pattern in
-                                                                    let uu___187
-                                                                    =
-                                                                    let uu___188
-                                                                    =
-                                                                    FStar_TypeChecker_NBETerm.e_list
-                                                                    FStar_Reflection_V2_NBEEmbeddings.e_binding in
-                                                                    FStar_TypeChecker_NBETerm.e_list
-                                                                    uu___188 in
-                                                                    FStar_TypeChecker_NBETerm.e_tuple2
-                                                                    uu___186
-                                                                    uu___187 in
                                                                     FStar_TypeChecker_NBETerm.e_option
-                                                                    uu___185 in
-                                                                    FStar_Tactics_V2_InterpFuns.mk_tac_step_4
-                                                                    Prims.int_zero
-                                                                    "check_match_complete"
-                                                                    FStar_Tactics_V2_Basic.refl_check_match_complete
-                                                                    FStar_Reflection_V2_Embeddings.e_env
-                                                                    FStar_Reflection_V2_Embeddings.e_term
-                                                                    FStar_Reflection_V2_Embeddings.e_term
-                                                                    uu___181
-                                                                    uu___182
-                                                                    FStar_Tactics_V2_Basic.refl_check_match_complete
-                                                                    FStar_Reflection_V2_NBEEmbeddings.e_env
-                                                                    FStar_Reflection_V2_NBEEmbeddings.e_term
-                                                                    FStar_Reflection_V2_NBEEmbeddings.e_term
+                                                                    FStar_Reflection_V2_NBEEmbeddings.e_universe in
+                                                                    let uu___184
+                                                                    =
+                                                                    FStar_TypeChecker_NBETerm.e_list
+                                                                    FStar_TypeChecker_NBETerm.e_issue in
+                                                                    FStar_TypeChecker_NBETerm.e_tuple2
                                                                     uu___183
                                                                     uu___184 in
+                                                                    FStar_Tactics_V2_InterpFuns.mk_tac_step_2
+                                                                    Prims.int_zero
+                                                                    "universe_of"
+                                                                    FStar_Tactics_V2_Basic.refl_universe_of
+                                                                    FStar_Reflection_V2_Embeddings.e_env
+                                                                    FStar_Reflection_V2_Embeddings.e_term
+                                                                    uu___181
+                                                                    FStar_Tactics_V2_Basic.refl_universe_of
+                                                                    FStar_Reflection_V2_NBEEmbeddings.e_env
+                                                                    FStar_Reflection_V2_NBEEmbeddings.e_term
+                                                                    uu___182 in
                                                                     let uu___181
                                                                     =
                                                                     let uu___182
@@ -2144,13 +2146,8 @@ let (uu___193 : unit) =
                                                                     =
                                                                     let uu___184
                                                                     =
-                                                                    let uu___185
-                                                                    =
-                                                                    FStar_Syntax_Embeddings.e_tuple2
-                                                                    FStar_Reflection_V2_Embeddings.e_term
-                                                                    FStar_Reflection_V2_Embeddings.e_term in
                                                                     FStar_Syntax_Embeddings.e_option
-                                                                    uu___185 in
+                                                                    FStar_Syntax_Embeddings.e_unit in
                                                                     let uu___185
                                                                     =
                                                                     FStar_Syntax_Embeddings.e_list
@@ -2162,13 +2159,8 @@ let (uu___193 : unit) =
                                                                     =
                                                                     let uu___185
                                                                     =
-                                                                    let uu___186
-                                                                    =
-                                                                    FStar_TypeChecker_NBETerm.e_tuple2
-                                                                    FStar_Reflection_V2_NBEEmbeddings.e_term
-                                                                    FStar_Reflection_V2_NBEEmbeddings.e_term in
                                                                     FStar_TypeChecker_NBETerm.e_option
-                                                                    uu___186 in
+                                                                    FStar_TypeChecker_NBETerm.e_unit in
                                                                     let uu___186
                                                                     =
                                                                     FStar_TypeChecker_NBETerm.e_list
@@ -2178,12 +2170,12 @@ let (uu___193 : unit) =
                                                                     uu___186 in
                                                                     FStar_Tactics_V2_InterpFuns.mk_tac_step_2
                                                                     Prims.int_zero
-                                                                    "instantiate_implicits"
-                                                                    FStar_Tactics_V2_Basic.refl_instantiate_implicits
+                                                                    "check_prop_validity"
+                                                                    FStar_Tactics_V2_Basic.refl_check_prop_validity
                                                                     FStar_Reflection_V2_Embeddings.e_env
                                                                     FStar_Reflection_V2_Embeddings.e_term
                                                                     uu___183
-                                                                    FStar_Tactics_V2_Basic.refl_instantiate_implicits
+                                                                    FStar_Tactics_V2_Basic.refl_check_prop_validity
                                                                     FStar_Reflection_V2_NBEEmbeddings.e_env
                                                                     FStar_Reflection_V2_NBEEmbeddings.e_term
                                                                     uu___184 in
@@ -2193,43 +2185,69 @@ let (uu___193 : unit) =
                                                                     =
                                                                     let uu___185
                                                                     =
-                                                                    let uu___186
-                                                                    =
-                                                                    FStar_Syntax_Embeddings.e_option
-                                                                    FStar_Tactics_Embedding.e_unfold_side in
-                                                                    let uu___187
-                                                                    =
                                                                     FStar_Syntax_Embeddings.e_list
-                                                                    FStar_Syntax_Embeddings.e_issue in
-                                                                    FStar_Syntax_Embeddings.e_tuple2
-                                                                    uu___186
-                                                                    uu___187 in
+                                                                    FStar_Reflection_V2_Embeddings.e_pattern in
                                                                     let uu___186
                                                                     =
                                                                     let uu___187
                                                                     =
-                                                                    FStar_TypeChecker_NBETerm.e_option
-                                                                    FStar_Tactics_Embedding.e_unfold_side_nbe in
                                                                     let uu___188
                                                                     =
+                                                                    FStar_Syntax_Embeddings.e_list
+                                                                    FStar_Reflection_V2_Embeddings.e_pattern in
+                                                                    let uu___189
+                                                                    =
+                                                                    let uu___190
+                                                                    =
+                                                                    FStar_Syntax_Embeddings.e_list
+                                                                    FStar_Reflection_V2_Embeddings.e_binding in
+                                                                    FStar_Syntax_Embeddings.e_list
+                                                                    uu___190 in
+                                                                    FStar_Syntax_Embeddings.e_tuple2
+                                                                    uu___188
+                                                                    uu___189 in
+                                                                    FStar_Syntax_Embeddings.e_option
+                                                                    uu___187 in
+                                                                    let uu___187
+                                                                    =
                                                                     FStar_TypeChecker_NBETerm.e_list
-                                                                    FStar_TypeChecker_NBETerm.e_issue in
+                                                                    FStar_Reflection_V2_NBEEmbeddings.e_pattern in
+                                                                    let uu___188
+                                                                    =
+                                                                    let uu___189
+                                                                    =
+                                                                    let uu___190
+                                                                    =
+                                                                    FStar_TypeChecker_NBETerm.e_list
+                                                                    FStar_Reflection_V2_NBEEmbeddings.e_pattern in
+                                                                    let uu___191
+                                                                    =
+                                                                    let uu___192
+                                                                    =
+                                                                    FStar_TypeChecker_NBETerm.e_list
+                                                                    FStar_Reflection_V2_NBEEmbeddings.e_binding in
+                                                                    FStar_TypeChecker_NBETerm.e_list
+                                                                    uu___192 in
                                                                     FStar_TypeChecker_NBETerm.e_tuple2
-                                                                    uu___187
-                                                                    uu___188 in
-                                                                    FStar_Tactics_V2_InterpFuns.mk_tac_step_3
+                                                                    uu___190
+                                                                    uu___191 in
+                                                                    FStar_TypeChecker_NBETerm.e_option
+                                                                    uu___189 in
+                                                                    FStar_Tactics_V2_InterpFuns.mk_tac_step_4
                                                                     Prims.int_zero
-                                                                    "maybe_relate_after_unfolding"
-                                                                    FStar_Tactics_V2_Basic.refl_maybe_relate_after_unfolding
+                                                                    "check_match_complete"
+                                                                    FStar_Tactics_V2_Basic.refl_check_match_complete
                                                                     FStar_Reflection_V2_Embeddings.e_env
                                                                     FStar_Reflection_V2_Embeddings.e_term
                                                                     FStar_Reflection_V2_Embeddings.e_term
                                                                     uu___185
-                                                                    FStar_Tactics_V2_Basic.refl_maybe_relate_after_unfolding
+                                                                    uu___186
+                                                                    FStar_Tactics_V2_Basic.refl_check_match_complete
                                                                     FStar_Reflection_V2_NBEEmbeddings.e_env
                                                                     FStar_Reflection_V2_NBEEmbeddings.e_term
                                                                     FStar_Reflection_V2_NBEEmbeddings.e_term
-                                                                    uu___186 in
+                                                                    uu___187
+                                                                    uu___188 in
                                                                     let uu___185
                                                                     =
                                                                     let uu___186
@@ -2238,8 +2256,13 @@ let (uu___193 : unit) =
                                                                     =
                                                                     let uu___188
                                                                     =
-                                                                    FStar_Syntax_Embeddings.e_option
+                                                                    let uu___189
+                                                                    =
+                                                                    FStar_Syntax_Embeddings.e_tuple2
+                                                                    FStar_Reflection_V2_Embeddings.e_term
                                                                     FStar_Reflection_V2_Embeddings.e_term in
+                                                                    FStar_Syntax_Embeddings.e_option
+                                                                    uu___189 in
                                                                     let uu___189
                                                                     =
                                                                     FStar_Syntax_Embeddings.e_list
@@ -2251,8 +2274,13 @@ let (uu___193 : unit) =
                                                                     =
                                                                     let uu___189
                                                                     =
-                                                                    FStar_TypeChecker_NBETerm.e_option
+                                                                    let uu___190
+                                                                    =
+                                                                    FStar_TypeChecker_NBETerm.e_tuple2
+                                                                    FStar_Reflection_V2_NBEEmbeddings.e_term
                                                                     FStar_Reflection_V2_NBEEmbeddings.e_term in
+                                                                    FStar_TypeChecker_NBETerm.e_option
+                                                                    uu___190 in
                                                                     let uu___190
                                                                     =
                                                                     FStar_TypeChecker_NBETerm.e_list
@@ -2262,12 +2290,12 @@ let (uu___193 : unit) =
                                                                     uu___190 in
                                                                     FStar_Tactics_V2_InterpFuns.mk_tac_step_2
                                                                     Prims.int_zero
-                                                                    "maybe_unfold_head"
-                                                                    FStar_Tactics_V2_Basic.refl_maybe_unfold_head
+                                                                    "instantiate_implicits"
+                                                                    FStar_Tactics_V2_Basic.refl_instantiate_implicits
                                                                     FStar_Reflection_V2_Embeddings.e_env
                                                                     FStar_Reflection_V2_Embeddings.e_term
                                                                     uu___187
-                                                                    FStar_Tactics_V2_Basic.refl_maybe_unfold_head
+                                                                    FStar_Tactics_V2_Basic.refl_instantiate_implicits
                                                                     FStar_Reflection_V2_NBEEmbeddings.e_env
                                                                     FStar_Reflection_V2_NBEEmbeddings.e_term
                                                                     uu___188 in
@@ -2277,9 +2305,93 @@ let (uu___193 : unit) =
                                                                     =
                                                                     let uu___189
                                                                     =
+                                                                    let uu___190
+                                                                    =
+                                                                    FStar_Syntax_Embeddings.e_option
+                                                                    FStar_Tactics_Embedding.e_unfold_side in
+                                                                    let uu___191
+                                                                    =
+                                                                    FStar_Syntax_Embeddings.e_list
+                                                                    FStar_Syntax_Embeddings.e_issue in
+                                                                    FStar_Syntax_Embeddings.e_tuple2
+                                                                    uu___190
+                                                                    uu___191 in
+                                                                    let uu___190
+                                                                    =
+                                                                    let uu___191
+                                                                    =
+                                                                    FStar_TypeChecker_NBETerm.e_option
+                                                                    FStar_Tactics_Embedding.e_unfold_side_nbe in
+                                                                    let uu___192
+                                                                    =
+                                                                    FStar_TypeChecker_NBETerm.e_list
+                                                                    FStar_TypeChecker_NBETerm.e_issue in
+                                                                    FStar_TypeChecker_NBETerm.e_tuple2
+                                                                    uu___191
+                                                                    uu___192 in
+                                                                    FStar_Tactics_V2_InterpFuns.mk_tac_step_3
+                                                                    Prims.int_zero
+                                                                    "maybe_relate_after_unfolding"
+                                                                    FStar_Tactics_V2_Basic.refl_maybe_relate_after_unfolding
+                                                                    FStar_Reflection_V2_Embeddings.e_env
+                                                                    FStar_Reflection_V2_Embeddings.e_term
+                                                                    FStar_Reflection_V2_Embeddings.e_term
+                                                                    uu___189
+                                                                    FStar_Tactics_V2_Basic.refl_maybe_relate_after_unfolding
+                                                                    FStar_Reflection_V2_NBEEmbeddings.e_env
+                                                                    FStar_Reflection_V2_NBEEmbeddings.e_term
+                                                                    FStar_Reflection_V2_NBEEmbeddings.e_term
+                                                                    uu___190 in
+                                                                    let uu___189
+                                                                    =
+                                                                    let uu___190
+                                                                    =
+                                                                    let uu___191
+                                                                    =
+                                                                    let uu___192
+                                                                    =
+                                                                    FStar_Syntax_Embeddings.e_option
+                                                                    FStar_Reflection_V2_Embeddings.e_term in
+                                                                    let uu___194
+                                                                    =
+                                                                    FStar_Syntax_Embeddings.e_list
+                                                                    FStar_Syntax_Embeddings.e_issue in
+                                                                    FStar_Syntax_Embeddings.e_tuple2
+                                                                    uu___192
+                                                                    uu___194 in
+                                                                    let uu___192
+                                                                    =
+                                                                    let uu___194
+                                                                    =
+                                                                    FStar_TypeChecker_NBETerm.e_option
+                                                                    FStar_Reflection_V2_NBEEmbeddings.e_term in
+                                                                    let uu___195
+                                                                    =
+                                                                    FStar_TypeChecker_NBETerm.e_list
+                                                                    FStar_TypeChecker_NBETerm.e_issue in
+                                                                    FStar_TypeChecker_NBETerm.e_tuple2
+                                                                    uu___194
+                                                                    uu___195 in
+                                                                    FStar_Tactics_V2_InterpFuns.mk_tac_step_2
+                                                                    Prims.int_zero
+                                                                    "maybe_unfold_head"
+                                                                    FStar_Tactics_V2_Basic.refl_maybe_unfold_head
+                                                                    FStar_Reflection_V2_Embeddings.e_env
+                                                                    FStar_Reflection_V2_Embeddings.e_term
+                                                                    uu___191
+                                                                    FStar_Tactics_V2_Basic.refl_maybe_unfold_head
+                                                                    FStar_Reflection_V2_NBEEmbeddings.e_env
+                                                                    FStar_Reflection_V2_NBEEmbeddings.e_term
+                                                                    uu___192 in
+                                                                    let uu___191
+                                                                    =
+                                                                    let uu___192
+                                                                    =
+                                                                    let uu___194
+                                                                    =
                                                                     FStar_Syntax_Embeddings.e_list
                                                                     FStar_Syntax_Embeddings.e_string in
-                                                                    let uu___190
+                                                                    let uu___195
                                                                     =
                                                                     FStar_TypeChecker_NBETerm.e_list
                                                                     FStar_TypeChecker_NBETerm.e_string in
@@ -2288,21 +2400,21 @@ let (uu___193 : unit) =
                                                                     "push_open_namespace"
                                                                     FStar_Tactics_V2_Basic.push_open_namespace
                                                                     FStar_Reflection_V2_Embeddings.e_env
-                                                                    uu___189
+                                                                    uu___194
                                                                     FStar_Reflection_V2_Embeddings.e_env
                                                                     FStar_Tactics_V2_Basic.push_open_namespace
                                                                     FStar_Reflection_V2_NBEEmbeddings.e_env
-                                                                    uu___190
+                                                                    uu___195
                                                                     FStar_Reflection_V2_NBEEmbeddings.e_env in
-                                                                    let uu___189
+                                                                    let uu___194
                                                                     =
-                                                                    let uu___190
+                                                                    let uu___195
                                                                     =
-                                                                    let uu___191
+                                                                    let uu___196
                                                                     =
                                                                     FStar_Syntax_Embeddings.e_list
                                                                     FStar_Syntax_Embeddings.e_string in
-                                                                    let uu___192
+                                                                    let uu___197
                                                                     =
                                                                     FStar_TypeChecker_NBETerm.e_list
                                                                     FStar_TypeChecker_NBETerm.e_string in
@@ -2312,63 +2424,63 @@ let (uu___193 : unit) =
                                                                     FStar_Tactics_V2_Basic.push_module_abbrev
                                                                     FStar_Reflection_V2_Embeddings.e_env
                                                                     FStar_Syntax_Embeddings.e_string
-                                                                    uu___191
+                                                                    uu___196
                                                                     FStar_Reflection_V2_Embeddings.e_env
                                                                     FStar_Tactics_V2_Basic.push_module_abbrev
                                                                     FStar_Reflection_V2_NBEEmbeddings.e_env
                                                                     FStar_TypeChecker_NBETerm.e_string
-                                                                    uu___192
+                                                                    uu___197
                                                                     FStar_Reflection_V2_NBEEmbeddings.e_env in
-                                                                    let uu___191
+                                                                    let uu___196
                                                                     =
-                                                                    let uu___192
+                                                                    let uu___197
                                                                     =
-                                                                    let uu___194
+                                                                    let uu___198
                                                                     =
                                                                     FStar_Syntax_Embeddings.e_list
                                                                     FStar_Syntax_Embeddings.e_string in
-                                                                    let uu___195
+                                                                    let uu___199
                                                                     =
-                                                                    let uu___196
+                                                                    let uu___200
                                                                     =
                                                                     FStar_Syntax_Embeddings.e_either
                                                                     FStar_Reflection_V2_Embeddings.e_bv
                                                                     FStar_Reflection_V2_Embeddings.e_fv in
                                                                     FStar_Syntax_Embeddings.e_option
-                                                                    uu___196 in
-                                                                    let uu___196
+                                                                    uu___200 in
+                                                                    let uu___200
                                                                     =
                                                                     FStar_TypeChecker_NBETerm.e_list
                                                                     FStar_TypeChecker_NBETerm.e_string in
-                                                                    let uu___197
+                                                                    let uu___201
                                                                     =
-                                                                    let uu___198
+                                                                    let uu___202
                                                                     =
                                                                     FStar_TypeChecker_NBETerm.e_either
                                                                     FStar_Reflection_V2_NBEEmbeddings.e_bv
                                                                     FStar_Reflection_V2_NBEEmbeddings.e_fv in
                                                                     FStar_TypeChecker_NBETerm.e_option
-                                                                    uu___198 in
+                                                                    uu___202 in
                                                                     FStar_Tactics_V2_InterpFuns.mk_tac_step_2
                                                                     Prims.int_zero
                                                                     "resolve_name"
                                                                     FStar_Tactics_V2_Basic.resolve_name
                                                                     FStar_Reflection_V2_Embeddings.e_env
-                                                                    uu___194
-                                                                    uu___195
+                                                                    uu___198
+                                                                    uu___199
                                                                     FStar_Tactics_V2_Basic.resolve_name
                                                                     FStar_Reflection_V2_NBEEmbeddings.e_env
-                                                                    uu___196
-                                                                    uu___197 in
-                                                                    let uu___194
+                                                                    uu___200
+                                                                    uu___201 in
+                                                                    let uu___198
                                                                     =
-                                                                    let uu___195
+                                                                    let uu___199
                                                                     =
-                                                                    let uu___196
+                                                                    let uu___200
                                                                     =
                                                                     FStar_Syntax_Embeddings.e_list
                                                                     FStar_Syntax_Embeddings.e_issue in
-                                                                    let uu___197
+                                                                    let uu___201
                                                                     =
                                                                     FStar_TypeChecker_NBETerm.e_list
                                                                     FStar_TypeChecker_NBETerm.e_issue in
@@ -2381,7 +2493,7 @@ let (uu___193 : unit) =
                                                                     is;
                                                                     FStar_Tactics_Monad.ret
                                                                     ())
-                                                                    uu___196
+                                                                    uu___200
                                                                     FStar_Syntax_Embeddings.e_unit
                                                                     (fun is
                                                                     ->
@@ -2389,9 +2501,15 @@ let (uu___193 : unit) =
                                                                     is;
                                                                     FStar_Tactics_Monad.ret
                                                                     ())
-                                                                    uu___197
+                                                                    uu___201
                                                                     FStar_TypeChecker_NBETerm.e_unit in
-                                                                    [uu___195] in
+                                                                    [uu___199] in
+                                                                    uu___197
+                                                                    ::
+                                                                    uu___198 in
+                                                                    uu___195
+                                                                    ::
+                                                                    uu___196 in
                                                                     uu___192
                                                                     ::
                                                                     uu___194 in
