src/tactics/FStar.Tactics.V2.Basic.fst
@@ -1440,10 +1440,10 @@ let _t_trefl (allow_guards:bool) (l : term) (r : term) : tac unit =
           // Note, from well-typedness of the goal, we already know ?u.ty <: ty
           let check_uvar_subtype u t =
             let env = { goal_env g with gamma = g.goal_ctx_uvar.ctx_uvar_gamma } in
-            match Core.compute_term_type_handle_guards env t false (fun _ _ -> true)
+            match Core.compute_term_type_handle_guards env t (fun _ _ -> true)
             with
             | Inr _ -> false
-            | Inl t_ty -> (
+            | Inl (_, t_ty) -> (  // ignoring effect, ghost is ok
               match Core.check_term_subtyping env ty t_ty with
               | Inl None -> //unconditional subtype
                 mark_uvar_as_already_checked u;
@@ -2206,14 +2206,53 @@ let refl_core_compute_term_type (g:env) (e:term) (eff:Core.tot_or_ghost) : tac (
            Rel.force_trivial_guard g
              {Env.trivial_guard with guard_f = NonTrivial guard};
            true in
-         match Core.compute_term_type_handle_guards g e must_tot gh with
-         | Inl t ->
+         match Core.compute_term_type_handle_guards g e gh with
+         | Inl (_, t) ->
            let t = refl_norm_type g t in
            dbg_refl g (fun _ ->
              BU.format2 "refl_core_compute_term_type for %s computed type %s\n"
                (Print.term_to_string e)
                (Print.term_to_string t));
            t
+         | Inr err ->
+           dbg_refl g (fun _ -> BU.format1 "refl_core_compute_term_type: %s\n" (Core.print_error err));
+           Errors.raise_error (Errors.Fatal_IllTyped, "core_compute_term_type failed: " ^ (Core.print_error err)) Range.dummyRange)
+  else ret (None, [unexpected_uvars_issue (Env.get_range g)])
+
+let maybe_promote (g:env) (eff:Core.tot_or_ghost) (t:typ) : (Core.tot_or_ghost & typ) =
+  let open FStar.TypeChecker.Core in
+  match eff with
+  | E_Total -> eff, t
+  | E_Ghost ->
+    let c = t |> mk_GTotal |> N.maybe_ghost_to_pure g in
+    match c.n with
+    | Total t -> E_Total, t
+    | GTotal t -> E_Ghost, t
+    | _ ->
+      Errors.raise_error
+        (Errors.Fatal_UnexpectedTerm,
+         BU.format1 "core.maybe_promote: a non tot/ghost computation %s"
+           (FStar.Syntax.Print.comp_to_string c)) Range.dummyRange
+
+let refl_core_compute_term_type2 (g:env) (e:term) : tac (option (Core.tot_or_ghost & typ) & issues) =
+  if no_uvars_in_g g &&
+     no_uvars_in_term e
+  then refl_typing_builtin_wrapper (fun _ ->
+         dbg_refl g (fun _ ->
+           BU.format1 "refl_core_compute_term_type: %s\n" (Print.term_to_string e));
+         let gh = fun g guard ->
+           Rel.force_trivial_guard g
+             {Env.trivial_guard with guard_f = NonTrivial guard};
+           true in
+         match Core.compute_term_type_handle_guards g e gh with
+         | Inl (eff, t) ->
+           let eff, t = maybe_promote g eff t in
+           let t = refl_norm_type g t in
+           dbg_refl g (fun _ ->
+             BU.format2 "refl_core_compute_term_type for %s computed type %s\n"
+               (Print.term_to_string e)
+               (Print.term_to_string t));
+           eff, t
          | Inr err ->
            dbg_refl g (fun _ -> BU.format1 "refl_core_compute_term_type: %s\n" (Core.print_error err));
            Errors.raise_error (Errors.Fatal_IllTyped, "core_compute_term_type failed: " ^ (Core.print_error err)) Range.dummyRange)
@@ -2279,8 +2318,8 @@ let refl_tc_term (g:env) (e:term) (eff:Core.tot_or_ghost) : tac (option (term & 
         Rel.force_trivial_guard g
           {Env.trivial_guard with guard_f = NonTrivial guard};
         true in
-     match Core.compute_term_type_handle_guards g e must_tot gh with
-     | Inl t ->
+     match Core.compute_term_type_handle_guards g e gh with
+     | Inl (_, t) ->
         let t = refl_norm_type g t in
         dbg_refl g (fun _ ->
           BU.format2 "refl_tc_term for %s computed type %s\n"
@@ -2290,6 +2329,61 @@ let refl_tc_term (g:env) (e:term) (eff:Core.tot_or_ghost) : tac (option (term & 
      | Inr err ->
         dbg_refl g (fun _ -> BU.format1 "refl_tc_term failed: %s\n" (Core.print_error err));
         Errors.raise_error (Errors.Fatal_IllTyped, "tc_term callback failed: " ^ Core.print_error err) e.pos
+    end
+    with
+    | Errors.Error (Errors.Error_UnexpectedUnresolvedUvar, _, _, _) ->
+      Errors.raise_error (Errors.Fatal_IllTyped, "UVars remaing in term after tc_term callback") e.pos)
+  else
+    ret (None, [unexpected_uvars_issue (Env.get_range g)])
+
+let refl_tc_term2 (g:env) (e:term) : tac (option (term & (Core.tot_or_ghost & typ)) & issues) =
+  if no_uvars_in_g g &&
+     no_uvars_in_term e
+  then refl_typing_builtin_wrapper (fun _ ->
+    dbg_refl g (fun _ ->
+      BU.format1 "refl_tc_term: %s\n" (Print.term_to_string e));
+    dbg_refl g (fun _ -> "refl_tc_term: starting tc {\n");
+    //
+    // we don't instantiate implicits at the end of e
+    // it is unlikely that we will be able to resolve them,
+    //   and refl typechecking API will fail if there are unresolved uvars
+    //
+    // note that this will still try to resolve implicits within e
+    // the typechecker does not check for this env flag for such implicits
+    //
+    let g = {g with instantiate_imp=false} in
+    //
+    // lax check to elaborate
+    //
+    let e =
+      let g = {g with phase1 = true; lax = true} in
+      let must_tot = true in
+      let e, _, guard = g.typeof_tot_or_gtot_term g e must_tot in
+      Rel.force_trivial_guard g guard;
+      e in
+    try
+     begin
+     let e = SC.deep_compress false e in
+     // TODO: may be should we check here that e has no unresolved implicits?
+     dbg_refl g (fun _ ->
+       BU.format1 "} finished tc with e = %s\n"
+         (Print.term_to_string e));
+     let gh = fun g guard ->
+        Rel.force_trivial_guard g
+          {Env.trivial_guard with guard_f = NonTrivial guard};
+        true in
+     match Core.compute_term_type_handle_guards g e gh with
+     | Inl (eff, t) ->
+       let eff, t = maybe_promote g eff t in
+       let t = refl_norm_type g t in
+       dbg_refl g (fun _ ->
+         BU.format2 "refl_tc_term for %s computed type %s\n"
+           (Print.term_to_string e)
+           (Print.term_to_string t));
+       e, (eff, t)
+     | Inr err ->
+       dbg_refl g (fun _ -> BU.format1 "refl_tc_term failed: %s\n" (Core.print_error err));
+       Errors.raise_error (Errors.Fatal_IllTyped, "tc_term callback failed: " ^ Core.print_error err) e.pos
     end
     with
     | Errors.Error (Errors.Error_UnexpectedUnresolvedUvar, _, _, _) ->
