src/tactics/FStar.Tactics.V2.Interpreter.fst
@@ -615,6 +615,10 @@ let () =
         refl_core_compute_term_type RE.e_env RE.e_term E.e_tot_or_ghost (e_tuple2 (e_option RE.e_term) (e_list e_issue))
         refl_core_compute_term_type NRE.e_env NRE.e_term E.e_tot_or_ghost_nbe NBET.(e_tuple2 (e_option NRE.e_term) (e_list e_issue));
 
+      mk_tac_step_2 0 "core_compute_term_type2"
+        refl_core_compute_term_type2 RE.e_env RE.e_term (e_tuple2 (e_option (e_tuple2 E.e_tot_or_ghost RE.e_term)) (e_list e_issue))
+        refl_core_compute_term_type2 NRE.e_env NRE.e_term NBET.(e_tuple2 (e_option (e_tuple2 E.e_tot_or_ghost_nbe NRE.e_term)) (e_list e_issue));
+
       mk_tac_step_4 0 "core_check_term"
         refl_core_check_term RE.e_env RE.e_term RE.e_term E.e_tot_or_ghost (e_tuple2 (e_option e_unit) (e_list e_issue))
         refl_core_check_term NRE.e_env NRE.e_term NRE.e_term E.e_tot_or_ghost_nbe NBET.(e_tuple2 (e_option e_unit) (e_list e_issue));
@@ -622,6 +626,10 @@ let () =
       mk_tac_step_3 0 "tc_term"
         refl_tc_term RE.e_env RE.e_term E.e_tot_or_ghost (e_tuple2 (e_option (e_tuple2 RE.e_term RE.e_term)) (e_list e_issue))
         refl_tc_term NRE.e_env NRE.e_term E.e_tot_or_ghost_nbe NBET.(e_tuple2 (e_option (e_tuple2 NRE.e_term NRE.e_term)) (e_list e_issue));
+
+      mk_tac_step_2 0 "tc_term2"
+        refl_tc_term2 RE.e_env RE.e_term (e_tuple2 (e_option (e_tuple2 RE.e_term (e_tuple2 E.e_tot_or_ghost RE.e_term))) (e_list e_issue))
+        refl_tc_term2 NRE.e_env NRE.e_term NBET.(e_tuple2 (e_option (e_tuple2 NRE.e_term (e_tuple2 E.e_tot_or_ghost_nbe NRE.e_term))) (e_list e_issue));
 
       mk_tac_step_2 0 "universe_of"
         refl_universe_of RE.e_env RE.e_term (e_tuple2 (e_option RE.e_universe) (e_list e_issue))
